Progress on preprocess.lean

src/smt/preprocess.lean
@@ -1,7 +1,36 @@
-import tactic.finish
+import tactic.finish tactic.tidy
 
 open expr
 namespace tactic
+
+section intro_ext
+
+meta def intro_ext_tactics : list (tactic string) :=
+[ tactic.reflexivity                                 >> pure "refl",
+  -- `[exact dec_trivial]                        >> pure "exact dec_trivial",
+  -- propositional_goal >> assumption            >> pure "assumption",
+  tidy.ext1_wrapper,
+  intros1                                     >>= λ ns, pure ("intros " ++ (" ".intercalate (ns.map (λ e, e.to_string)))),
+  -- auto_cases,
+  -- `[apply_auto_param]                         >> pure "apply_auto_param",
+  -- `[dsimp at *]                               >> pure "dsimp at *",
+  -- `[simp at *]                                >> pure "simp at *",
+  -- fsplit                                      >> pure "fsplit",
+  -- injections_and_clear                        >> pure "injections_and_clear",
+  -- propositional_goal >> (`[solve_by_elim])    >> pure "solve_by_elim",
+  -- `[unfold_aux]                               >> pure "unfold_aux",
+  tidy.run_tactics ]
+
+meta def intro_ext_cfg : tidy.cfg := {tactics := intro_ext_tactics}
+
+-- example : (λ x : ℕ, x + 1) = λ x, 0 + x + 0 + 1  :=
+-- begin
+--  tidy? intro_ext_cfg,
+-- end
+
+end intro_ext
+
+section lambda_lifting
 
 /-- Given an expr f of the form λ x, body and an expr e, return the expr
     ∀ x, e x = body -/
@@ -17,9 +46,12 @@ protected meta def axiom_of_lambda (e : expr) : expr → tactic expr
   | (elet a b c d) := return $ elet a b c d
   | (macro a b) := return $ macro a b
 
+meta def trace_goal_raw : tactic unit :=
+  target >>= tactic.trace ∘ to_raw_fmt
+
 protected meta def lambda_set_core (a h : name) (v : expr) : tactic unit :=
-do tp <- infer_type v,
-   nv ← definev a tp v,
+do -- tp <- infer_type v,
+   nv ← pose a none v,
    e <- (tactic.axiom_of_lambda nv v),
    trace e,
    axm ← (tactic.axiom_of_lambda nv v) >>= assert h,
@@ -37,8 +69,8 @@ do tp <- infer_type v,
      -- trace h,
      -- tactic.dsimp_target s []
      -- hyps.mmap (λ h, simp_hyp s [] h),
-     -- trace "simp_hyp succeeded",
-     interactive.simp_core_aux {} tactic.failed s [] [h] tt,
+     trace "simp_hyp succeeded",
+     tactic.try $ interactive.simp_core_aux {} (tactic.failed) s [] [h] tt,
      tgt <- (target >>= pp),
      trace ("target after simp call is now... \n ⊢ " ++ (to_string (tgt)))
 
@@ -49,11 +81,17 @@ meta def lambda_set : expr → tactic unit
   | (mvar a b c) := lambda_set c
   | (local_const a b c d) := lambda_set d 
   | (app a b) := lambda_set a >> lambda_set b
-  | (lam a b c d) := do n <- (tactic.get_unused_name "HEWWO"),
+  | (lam a b c d) := tidy intro_ext_cfg >> -- trace_goal_raw >> trace "tidy was called" >>
+  (target >>= lambda_set) <|> tidy intro_ext_cfg <|>
+                    fail_if_no_goals >>
+                    -- trace_goal_raw >>
+                    do n <- (tactic.get_unused_name "HEWWO"),
                         n' <- (tactic.get_unused_name "HERRO"),
                         tactic.trace "lambda_set_core is being called again",
                         tactic.lambda_set_core n n' (lam a b c d)
-  | (pi a b c d) := return ()
+  | (pi a b c d) := -- tidy intro_ext_cfg >> trace "tidy was called'" >>  target >>= lambda_set <|> fail_if_no_goals
+                    -- >>  
+                    lambda_set c >> lambda_set d
   -- (tactic.get_unused_name) >>= tactic.intro >>= lambda_set
                      -- do n <- (tactic.get_unused_name),
                      --    n' <- (tactic.get_unused_name "HEWWO"),
@@ -66,13 +104,12 @@ meta def trace_intro : tactic unit :=
   do e <- (tactic.get_unused_name "H") >>= tactic.intro,
   tactic.trace e.to_raw_fmt
 
-meta def lambda_set_tactic : tactic unit := do tgt <- target, lambda_set tgt
- 
-#check tactic.interactive.dsimp
+meta def lambda_set_tactic : tactic unit := target >>= lambda_set
 
+-- tidy intro_ext_cfg >> (target >>= lambda_set)
 example : (λ x : ℕ, x + 1) = λ x, 0 + x + 0 + 1  :=
 begin
-  lambda_set_tactic, simp[HEWWO, HEWWO_1],
+  lambda_set_tactic, simp
 
 /- tactic state is now
   HEWWO : ℕ → ℕ := λ (x : ℕ), x + 1,
@@ -86,21 +123,108 @@ begin
 end
 
 /-
-Note: the call to the simplifier annoying simplifies other parts of the target along with the intended rewrite. Possible fix: using rw instead of simp? Or use expr.replace and then change?
+Note: the call to the simplifier annoyingly simplifies other parts of the target along with the intended rewrite. Possible fix: using rw instead of simp? Or use expr.replace and then change?
 
-Also todo: hook this up to a fragment of tidy or chain, to keep trying to apply extensionality lemmas. The example above is vacuous because we can get rid of the lambdas with funext
+Also todo: hook this up to a fragment of tidy or chain, to keep trying to apply extensionality lemmas. The example above is vacuous because we can get rid of the lambdas with funext. After `chain` is finished, use `expr.is_sort` to check if there are any quantifications over sorts
+
+In case we have assumptions with universal quantifications over types, we should also populate a list with all types which occur in the initial goal, plus types relevant to the target logic, with which to instantiate such quantifications
 -/
-end tactic
 
-meta def expr.is_type : expr → bool
-| (sort zero) := ff
--- | (sort $ level.succ l) := tt
-| (var _) := ff
-| (const _ _) := ff
-| (mvar _ _ _) := ff
-| (local_const _ _ _ _) := ff
-| (app _ _) := ff
-| (lam _ _ _ _) := ff
-| (pi _ _ _ _) := ff
-| (elet _ _ _ _) := ff
-| (macro _ _) := ff
+end lambda_lifting
+
+section is_first_order
+
+/- Checks if an an expr contains a quantification over types -/
+meta def contains_type_variables : expr → bool
+  | (lam a b c d) := is_sort c ∨ contains_type_variables d
+  | (var n) := ff
+  | (sort l) := ff
+  | (const a b) := ff
+  | (mvar a b c) := contains_type_variables c
+  | (local_const a b c d) := contains_type_variables d
+  | (app a b) := contains_type_variables a ∨ contains_type_variables b
+  | (pi a b c d) := is_sort c ∨ contains_type_variables d
+  | (elet a b c d) := is_sort c ∨ contains_type_variables b ∨ contains_type_variables d
+  | (macro a b) := (b.map contains_type_variables).foldr (λ x y, x ∨ y) ff
+
+meta def contains_lambda : expr → bool
+  | (lam a b c d) := tt
+  | (var n) := ff
+  | (sort l) := ff
+  | (const a b) := ff
+  | (mvar a b c) := contains_lambda c
+  | (local_const a b c d) := contains_lambda d
+  | (app a b) := contains_lambda a ∨ contains_lambda b
+  | (pi a b c d) := contains_lambda c ∨ contains_lambda d
+  | (elet a b c d) := contains_lambda c ∨ contains_lambda b ∨ contains_lambda d
+  | (macro a b) := (b.map contains_lambda).foldr (λ x y, x ∨ y) ff
+
+meta def is_first_order : expr → bool := λ e, ¬ (contains_lambda e ∨ contains_type_variables e)
+
+meta def is_first_order_goal : tactic bool := target >>= (λ e, (return $ is_first_order e))
+
+meta def is_first_order_goal_trace : tactic unit := is_first_order_goal >>= tactic.trace
+
+-- example : (λ x : ℕ, x + 1) = λ x, 0 + x + 0 + 1  :=
+-- begin
+--  tidy? intro_ext_cfg, is_first_order_goal_trace
+-- end
+
+end is_first_order
+
+section type_scraper
+
+/-- Insert a into xs if a is not in xs -/
+/- We use this to avoid duplicate types when instantiating -/
+def cons_new {α : Type*} [decidable_eq α] (a : α) (xs : list α) : list α :=
+  if a ∈ xs then xs else a :: xs
+
+local infix `::'`:50 := cons_new
+
+/-- Return a list of types which occur in the expr e -/
+meta def types_in_expr  : expr →  tactic (list expr)
+  | (lam a b c d) := do xs <- (types_in_expr d), return (c::'xs)
+  | (var n) := return []
+  | (sort l) := return []
+  | (const a b) := return []
+  | (mvar a b c) := types_in_expr c
+  | (local_const a b c d) := types_in_expr d
+  | (app a b) := do xs <- types_in_expr a, ys <- types_in_expr b, return (xs ++ ys)
+  | (pi a b c d) := do xs <- (types_in_expr d), return (c::'xs)
+  | (elet a b c d) := do xs <- types_in_expr b, ys <- types_in_expr d, return $ c::'(xs ++ ys)
+  | (macro a b) := (b.map types_in_expr).mfoldr (λ x y, do x' <- x, return (x' ++ y)) []
+
+meta def types_in_goal : tactic unit :=
+  target >>= types_in_expr >>= tactic.trace
+
+-- example : ∀ p : Prop, ∀ q : Prop, p ∧ q ↔ q ∧ p  :=
+-- begin
+--   types_in_goal,
+-- end
+end type_scraper
+
+section preprocessor -- TODO
+-- intended behavior: user calls it once and it attempts to perform rudimentary preprocessing and lambda-lifting. It fails if, at the end, the goal contains lambdas or pis. It will also attempt to instantiate quantifications over types in the assumptions if they are introduced.
+
+meta def preprocess : tactic unit :=
+do tgt                <- target,
+   instantiation_list <- types_in_expr tgt
+    -- trace instantiation_list
+   >> lambda_set_tactic,
+   do first_order_goal_flag <- is_first_order_goal,
+      if first_order_goal_flag then return () else tactic.trace "Preprocessing failed, target is not first-order"
+
+example : ∀ f : ℕ → ℕ, ∀ g : ℕ → ℕ → ℕ, (g $ f 0 ) 0 = (λ x y, g x y) (f 0) 0 ∧ ∀ p q : ℕ → Prop, ∀ r : Prop, (p 0) ↔ r ↔ ∀ r : Prop, (q 0) ↔ r
+:=
+begin
+  preprocess, tidy, sorry
+end
+
+example : (λ x : ℕ, x + 1) = λ x, 0 + x + 0 + 1  :=
+begin preprocess, simp end
+
+-- TODO perform instantiations using congr_fun after applying extensionality lemmas
+
+end preprocessor
+  
+end tactic
